theories/Synthetic/Models_Equivalent.v
@@ -16,9 +16,11 @@ From Undecidability Require Import
   Diophantine
   Diophantine_to_MuRec_computable
   MuRec_computable_to_L_computable
-  L_computable_to_TM_computable
-  L_computable_to_MMA_computable
-  MMA_computable_to_TM_computable.
+  L_computable_closed_to_MMA_computable
+  MMA_computable_to_TM_computable
+  MMA_computable_to_L_computable_closed
+  MM_computable_to_MMA_computable
+  ClosedLAdmissible.
 
 Theorem equivalence {k} (R : Vector.t nat k -> nat -> Prop) :
   (TM_computable R -> BSM_computable R) /\
@@ -27,8 +29,11 @@ Theorem equivalence {k} (R : Vector.t nat k -> nat -> Prop) :
   (FRACTRAN_computable R -> Diophantine' R /\ functional R) /\
   (Diophantine' R /\ functional R -> MuRec_computable R) /\
   (MuRec_computable R -> L_computable R) /\
-  (L_computable R -> MMA_computable R) /\
-  (MMA_computable R -> TM_computable R).
+  (L_computable_closed R -> MMA_computable R) /\
+  (MMA_computable R -> TM_computable R) /\
+  (MMA_computable R -> L_computable_closed R) /\
+  (MM_computable R -> MMA_computable R) /\
+  (L_computable R -> L_computable_closed R).
 Proof.
   repeat split.
   - apply TM_computable_to_BSM_computable.
@@ -38,6 +43,9 @@ Proof.
   - intros ? ? ? ? ?. eapply FRACTRAN_computable.FRACTRAN_computable_functional; eauto.
   - intros []. eapply Diophantine_to_MuRec_computable; eauto.
   - apply MuRec_computable_to_L_computable.
-  - apply L_computable_to_MMA_computable.
+  - apply L_computable_closed_to_MMA_computable.
   - apply MMA_computable_to_TM_computable.
+  - apply MMA_computable_to_L_computable_closed.
+  - apply MM_computable_to_MMA_computable.
+  - apply L_computable_can_closed.
 Qed.
