theories/TM/Reductions/HaltLclosed_to_HaltTM_5.v
@@ -2,15 +2,13 @@ From Undecidability Require Import
   L.L TM.TM Synthetic.Definitions Synthetic.ReducibilityFacts.
 
 From Undecidability Require 
-  L.Reductions.HaltL_to_HaltLclosed
   LambdaCalculus.Reductions.HaltLclosed_to_wCBNclosed
   LambdaCalculus.Reductions.wCBNclosed_to_KrivineMclosed_HALT
   MinskyMachines.Reductions.KrivineMclosed_HALT_to_MMA_HALTING
   TM.Reductions.MMA_HALTING_n_to_HaltTM_n.
 
-Lemma reduction : HaltL ⪯ HaltTM 5.
+Lemma reduction : HaltLclosed ⪯ HaltTM 5.
 Proof.
-  apply (reduces_transitive HaltL_to_HaltLclosed.reduction).
   apply (reduces_transitive HaltLclosed_to_wCBNclosed.reduction).
   apply (reduces_transitive wCBNclosed_to_KrivineMclosed_HALT.reduction).
   apply (reduces_transitive KrivineMclosed_HALT_to_MMA_HALTING.reduction).
